tutorial/utp_csp_buffer.thy
@@ -1,89 +1,73 @@
-section {* Simple Buffer in UTP CSP *}
+section \<open> Simple Buffer in UTP CSP \<close>
 
 theory utp_csp_buffer
   imports "UTP-Circus.utp_circus"
 begin
 
-subsection {* Definitions *}
+subsection \<open> Definitions \<close>
 
-text {* A stateful CSP (Circus) process is parametrised over two alphabets: one for the state-space,
+text \<open> A stateful CSP (Circus) process is parametrised over two alphabets: one for the state-space,
   which consists of the state variables, and one for events, which consists of channels. We first
   define the statespace using the \textbf{alphabet} command. The single state variable $buf$ is
-  a list of natural numbers that is currently in the buffer. *}
+  a list of natural numbers that is currently in the buffer. \<close>
 
 alphabet st_buffer =
   buff :: "nat list"
 
-text {* Channels are created using the \textbf{datatype} command. In this case we can either input
-  a value to go in the buffer, or output one presently in the buffer. *}
+text \<open> Channels are created using the \textbf{datatype} command. In this case we can either input
+  a value to go in the buffer, or output one presently in the buffer. \<close>
 
 datatype ch_buffer =
   inp nat | outp nat
 
-text {* We create a useful type to describe an action of the buffer as a CSP action parametrised
-  by the state and event alphabet. *}
+text \<open> We create a useful type to describe an action of the buffer as a CSP action parametrised
+  by the state and event alphabet. \<close>
 
 type_synonym act_buffer = "(st_buffer, ch_buffer) action"
 
-text {* We define the main body of behaviour for the buffer as an abbreviation. We can either
+text \<open> We define an action that initialises the buffer state by setting it to empty. \<close>
+
+abbreviation Init :: act_buffer where
+"Init \<equiv> buff :=\<^sub>C \<langle>\<rangle>"
+
+text \<open> We define the main body of behaviour for the buffer as an abbreviation. We can either
   input a value and then place it into the buffer, or else, provided that the buffer is non-empty,
-  we can output a value presently in the buffer. *}
+  we can output a value presently in the buffer. \<close>
 
 abbreviation DoBuff :: act_buffer where
 "DoBuff \<equiv> (inp?(v) \<^bold>\<rightarrow> buff :=\<^sub>C (&buff ^\<^sub>u \<langle>\<guillemotleft>v\<guillemotright>\<rangle>)
            \<box> (#\<^sub>u(&buff) >\<^sub>u 0) &\<^sub>u outp!(head\<^sub>u(&buff)) \<^bold>\<rightarrow> buff :=\<^sub>C tail\<^sub>u(&buff))"
 
-text {* The main action of the buffer first initialises the single state variable $buff$, and
-  enters a recursive loop where it does \emph{DoBuff} over and over. *}
+text \<open> The main action of the buffer first initialises the single state variable $buff$, and
+  enters a recursive loop where it does \emph{DoBuff} over and over. \<close>
 
 definition Buffer :: act_buffer where
-[rdes]: "Buffer = buff :=\<^sub>C \<langle>\<rangle> ;; (\<mu>\<^sub>C X \<bullet> DoBuff ;; X)"
+[rdes_def]: "Buffer = Init ;; while\<^sub>R true do DoBuff od"
 
-subsection {* Calculations *}
+subsection \<open> Calculations \<close>
 
-text {* The precondition of the main body is true because no divergence is possible. We calculate
-  this using the reactive design calculation tactic, \textbf{rdes-calc}. *}
-  
-lemma preR_DoBuff: "pre\<^sub>R(DoBuff) = true\<^sub>r"
-  by (rdes_calc)
+text \<open> The @{term Init} action is represented by a simple contract with a true precondition,
+  false pericondition (i.e. there is no intermediate behaviour), and finally sets the state
+  variable to be empty, whilst leaving the state unchanged. There are no constraints on
+  the initial state. \<close>
 
-text {* The pericondition ensures that no input on channel $inp$ is being refused, the trace
-  stays the same (no event has yet occurred), and provided the buffer is non-empty then outputting
-  the head of the buffer is not refused either. *}
+lemma Init_contract:
+  "Init = \<^bold>R\<^sub>s(true\<^sub>r \<turnstile> false \<diamondop> \<Phi>(true,[&buff \<mapsto>\<^sub>s \<langle>\<rangle>],\<langle>\<rangle>))"
+  by (rdes_simp)
 
-lemma periR_DoBuff:
-  "peri\<^sub>R(DoBuff) =
-     ((\<Squnion> v \<bullet> (inp\<cdot>\<guillemotleft>v\<guillemotright>)\<^sub>u \<notin>\<^sub>u $ref\<acute>) \<and> $tr\<acute> =\<^sub>u $tr \<and>
-      (#\<^sub>u($st:buff) >\<^sub>u 0 \<Rightarrow> \<lceil>(outp\<cdot>head\<^sub>u(&buff))\<^sub>u\<rceil>\<^sub>S\<^sub>< \<notin>\<^sub>u $ref\<acute>))"
-  by (rdes_calc, rel_auto)
+lemma DoBuff_contract:
+  "DoBuff = \<^bold>R\<^sub>s (true\<^sub>r \<turnstile>
+                \<E>(true,\<langle>\<rangle>, (\<Sqinter> x \<bullet> {(inp\<cdot>\<guillemotleft>x\<guillemotright>)\<^sub>u}\<^sub>u) \<union>\<^sub>u ({(outp\<cdot>head\<^sub>u(&buff))\<^sub>u}\<^sub>u \<triangleleft> 0 <\<^sub>u #\<^sub>u(&buff) \<triangleright> {}\<^sub>u)) \<diamondop>
+                ((\<Sqinter> x \<bullet> \<Phi>(true,[&buff \<mapsto>\<^sub>s &buff ^\<^sub>u \<langle>\<guillemotleft>x\<guillemotright>\<rangle>],\<langle>(inp\<cdot>\<guillemotleft>x\<guillemotright>)\<^sub>u\<rangle>)) \<or>
+                 \<Phi>(0 <\<^sub>u #\<^sub>u(&buff), [&buff \<mapsto>\<^sub>s tail\<^sub>u(&buff)], \<langle>(outp\<cdot>head\<^sub>u(&buff))\<^sub>u\<rangle>)))"
+  by (rdes_eq)
 
-text {* The postcondition has two possibilities. In the first option a particular input $v$ was
-  received and so the trace was extended, and the $buff$ variable is extended with $v$. In the second
-  option the buffer is non-empty, the trace is extended to output the value at the head, and the head
-  is removed from the buffer. *}
-
-lemma postR_DoBuff:
-  "post\<^sub>R(DoBuff) = ((\<Sqinter> v \<bullet> \<Phi>(true,[buff \<mapsto>\<^sub>s &buff ^\<^sub>u \<langle>\<guillemotleft>v\<guillemotright>\<rangle>],\<langle>(inp\<cdot>\<guillemotleft>v\<guillemotright>)\<^sub>u\<rangle>)) \<or>
-                    [0 <\<^sub>u #\<^sub>u(&buff)]\<^sub>S\<^sub>< \<and> \<Phi>(true,[buff \<mapsto>\<^sub>s tail\<^sub>u(&buff)],\<langle>(outp\<cdot>head\<^sub>u(&buff))\<^sub>u\<rangle>))"
-  by (rdes_calc, rel_auto)
-
-text {* The precondition of the overall buffer is again true as no divergence can occur. *}
-
-lemma preR_Buffer: "pre\<^sub>R(Buffer) = true\<^sub>r"
-  by rdes_calc
-
-text {* The postcondition is false as it is a non-terminating process. *}
-
-lemma postR_Buffer: "post\<^sub>R(Buffer) = false"
-  by rdes_calc
-
-text {* The pericondition is where the main behaviour of the buffer appears. Essentially this repeats
-  the postcondition of the main body again and again, each time finishing in the pericondition. We do
-  not reproduce it as it is a little long, but the calculation can be seen in Isabelle. *}
-
-lemma periR_Buffer: "peri\<^sub>R(Buffer) = undefined"
-    apply (simp add: Buffer_def rdes closure wp unrest rpred usubst alpha seq_UINF_distr)
-oops
-
+lemma Buffer_contract:
+  "Buffer = \<^bold>R\<^sub>s(true\<^sub>r \<turnstile> \<Phi>(true,[&buff \<mapsto>\<^sub>s \<langle>\<rangle>],\<langle>\<rangle>) ;;
+                       ((\<Sqinter> x \<bullet> \<Phi>(true, [&buff \<mapsto>\<^sub>s &buff ^\<^sub>u \<langle>\<guillemotleft>x\<guillemotright>\<rangle>], \<langle>(inp\<cdot>\<guillemotleft>x\<guillemotright>)\<^sub>u\<rangle>)) \<or>
+                        \<Phi>(0 <\<^sub>u #\<^sub>u(&buff), [&buff \<mapsto>\<^sub>s tail\<^sub>u(&buff)], \<langle>(outp\<cdot>head\<^sub>u(&buff))\<^sub>u\<rangle>))\<^sup>\<star>\<^sup>r ;;
+                        \<E>(true,\<langle>\<rangle>, (\<Sqinter> x \<bullet> {(inp\<cdot>\<guillemotleft>x\<guillemotright>)\<^sub>u}\<^sub>u) \<union>\<^sub>u ({(outp\<cdot>head\<^sub>u(&buff))\<^sub>u}\<^sub>u \<triangleleft> 0 <\<^sub>u #\<^sub>u(&buff) \<triangleright> {}\<^sub>u)) \<diamondop>
+                       false)"
+  by (rdes_eq)
 
 end
