tutorial/utp_csp_ex.thy
@@ -1,7 +1,7 @@
 section {* CSP process examples *}
 
 theory utp_csp_ex
-  imports "../theories/utp_csp"
+  imports "../theories/circus/utp_circus"
 begin
 
 subsection {* Sequential Examples *}
@@ -9,7 +9,7 @@ subsection {* Sequential Examples *}
 text {* In this theory we calculate reactive designs for a number of simple CSP processes. *}
 
 lemma csp_ex_1:
-  "(a \<^bold>\<rightarrow> Skip) = \<^bold>R\<^sub>s(true \<turnstile> (&tt =\<^sub>u \<langle>\<rangle> \<and> \<guillemotleft>a\<guillemotright> \<notin>\<^sub>u $ref\<acute>) \<diamondop> (&tt =\<^sub>u \<langle>\<guillemotleft>a\<guillemotright>\<rangle> \<and> $st\<acute> =\<^sub>u $st))"
+  "(a \<^bold>\<rightarrow> Skip) = \<^bold>R\<^sub>s(true\<^sub>r \<turnstile> (&tt =\<^sub>u \<langle>\<rangle> \<and> \<guillemotleft>a\<guillemotright> \<notin>\<^sub>u $ref\<acute>) \<diamondop> (&tt =\<^sub>u \<langle>\<guillemotleft>a\<guillemotright>\<rangle> \<and> $st\<acute> =\<^sub>u $st))"
   by (simp add: PrefixCSP_RHS_tri closure rdes usubst, rel_auto)
 
 lemma csp_ex_2:
@@ -18,12 +18,12 @@ lemma csp_ex_2:
 
 lemma csp_ex_3:
   "(a \<^bold>\<rightarrow> b \<^bold>\<rightarrow> Skip)
-   = \<^bold>R\<^sub>s(true \<turnstile> (&tt =\<^sub>u \<langle>\<rangle> \<and> \<guillemotleft>a\<guillemotright> \<notin>\<^sub>u $ref\<acute> \<or> &tt =\<^sub>u \<langle>\<guillemotleft>a\<guillemotright>\<rangle> \<and> \<guillemotleft>b\<guillemotright> \<notin>\<^sub>u $ref\<acute>) \<diamondop> (&tt =\<^sub>u \<langle>\<guillemotleft>a\<guillemotright>,\<guillemotleft>b\<guillemotright>\<rangle> \<and> $st\<acute> =\<^sub>u $st))"
+   = \<^bold>R\<^sub>s(true\<^sub>r \<turnstile> (&tt =\<^sub>u \<langle>\<rangle> \<and> \<guillemotleft>a\<guillemotright> \<notin>\<^sub>u $ref\<acute> \<or> &tt =\<^sub>u \<langle>\<guillemotleft>a\<guillemotright>\<rangle> \<and> \<guillemotleft>b\<guillemotright> \<notin>\<^sub>u $ref\<acute>) \<diamondop> (&tt =\<^sub>u \<langle>\<guillemotleft>a\<guillemotright>,\<guillemotleft>b\<guillemotright>\<rangle> \<and> $st\<acute> =\<^sub>u $st))"
   by (subst PrefixCSP_RHS_tri, simp_all add: closure rdes usubst unrest, rel_auto)
 
 lemma csp_ex_4:
   "(a \<^bold>\<rightarrow> Stop \<box> b \<^bold>\<rightarrow> Skip) =
-       \<^bold>R\<^sub>s(true \<turnstile> (($tr\<acute> =\<^sub>u $tr \<and> \<guillemotleft>a\<guillemotright> \<notin>\<^sub>u $ref\<acute> \<and> \<guillemotleft>b\<guillemotright> \<notin>\<^sub>u $ref\<acute>) \<or> ($tr\<acute> =\<^sub>u $tr ^\<^sub>u \<langle>\<guillemotleft>a\<guillemotright>\<rangle>))
+       \<^bold>R\<^sub>s(true\<^sub>r \<turnstile> (($tr\<acute> =\<^sub>u $tr \<and> \<guillemotleft>a\<guillemotright> \<notin>\<^sub>u $ref\<acute> \<and> \<guillemotleft>b\<guillemotright> \<notin>\<^sub>u $ref\<acute>) \<or> ($tr\<acute> =\<^sub>u $tr ^\<^sub>u \<langle>\<guillemotleft>a\<guillemotright>\<rangle>))
                \<diamondop> ($tr\<acute> =\<^sub>u $tr ^\<^sub>u \<langle>\<guillemotleft>b\<guillemotright>\<rangle> \<and> $st\<acute> =\<^sub>u $st))"
   by (simp add: PrefixCSP_RHS_tri extChoice_tri_rdes rdes closure usubst unrest rpred, rel_auto)
 
