tutorial/utp_csp_pump.thy
@@ -1,7 +1,7 @@
 section {* Fuel Pump in UTP CSP *}
 
 theory utp_csp_pump
-  imports "../theories/utp_csp"
+  imports "../theories/circus/utp_circus"
 begin
 
 alphabet st_pump =
@@ -14,24 +14,24 @@ type_synonym op_pump = "st_pump hrel_des"
 type_synonym act_pump = "(st_pump, ch_pump) action"
 
 definition PInit :: "act_pump" where
-[urel_defs]: "PInit = (fuelQ :=\<^sub>C 5000)"
+[rdes_def]: "PInit = (fuelQ :=\<^sub>C 5000)"
 
 definition Reload :: "nat \<Rightarrow> act_pump" where
-[urel_defs]: "Reload(q) = fuelQ :=\<^sub>C (&fuelQ + \<guillemotleft>q\<guillemotright>)"
+[rdes_def]: "Reload(q) = fuelQ :=\<^sub>C (&fuelQ + \<guillemotleft>q\<guillemotright>)"
 
 definition Supply :: "nat \<Rightarrow> act_pump" where
-[urel_defs]: "Supply(q) = fuelQ :=\<^sub>C (&fuelQ - \<guillemotleft>q\<guillemotright>)"
+[rdes_def]: "Supply(q) = fuelQ :=\<^sub>C (&fuelQ - \<guillemotleft>q\<guillemotright>)"
 
 definition PumpActive :: "act_pump" where
-[urel_defs]: "PumpActive = putNozzle \<^bold>\<rightarrow> Skip \<box>
+[rdes_def]: "PumpActive = putNozzle \<^bold>\<rightarrow> Skip \<box>
                            enterAmount?(q) \<^bold>\<rightarrow> pressTrigger \<^bold>\<rightarrow> Supply(q) ;; releaseTrigger \<^bold>\<rightarrow> Skip"
 
 definition PumpIdle :: "act_pump" where
-[urel_defs]: "PumpIdle = liftNozzle \<^bold>\<rightarrow> PumpActive \<box>
+[rdes_def]: "PumpIdle = liftNozzle \<^bold>\<rightarrow> PumpActive \<box>
                          reload?(q) \<^bold>\<rightarrow> Reload(q) \<box>
                          init \<^bold>\<rightarrow> PInit"
 
 definition Pump :: "act_pump" where
-"Pump = init \<^bold>\<rightarrow> PInit ;; (\<mu> X \<bullet> PumpIdle ;; X)"
+[rdes_def]: "Pump = init \<^bold>\<rightarrow> PInit ;; (while\<^sub>R true do PumpIdle od)"
 
 end
